theories/logrel/ftlr_nop.v
@@ -40,7 +40,7 @@ Lemma ftlr_nop {i trans' mem_acc_tx ai regs ps_acc p_tx p_rx ps_na instr} trans 
                       LB@ i := [ps_na] -∗
                       transaction_hpool_global_transferred a1 -∗
                       transaction_pagetable_entries_transferred i a1 -∗
-                      retrieval_entries i a1 -∗
+                      retrieval_entries_transferred i a1 -∗
                       R0 @@ V0 ->r encode_hvc_func Run -∗
                       R1 @@ V0 ->r encode_vmid i -∗
                       RX_state@i:= a2 -∗
@@ -49,6 +49,7 @@ Lemma ftlr_nop {i trans' mem_acc_tx ai regs ps_acc p_tx p_rx ps_na instr} trans 
                       VMProp i (vmprop_unknown i p_tx p_rx trans') 1 -∗
                       transaction_pagetable_entries_owned i a1 -∗
                       pagetable_entries_excl_owned i (a0 ∖ {[p_rx; p_tx]} ∖ pages_in_trans a1) -∗
+                      retrieval_entries_owned i a1 -∗
                       (∃ mem : lang.mem, memory_pages (a0 ∪ pages_in_trans (trans_memory_in_trans i a1)) mem) -∗
                       WP ExecI @ i {{ _, True }}) -∗
    ([∗ map] r↦w ∈ regs, r @@ i ->r w) -∗
@@ -59,7 +60,7 @@ Lemma ftlr_nop {i trans' mem_acc_tx ai regs ps_acc p_tx p_rx ps_na instr} trans 
    LB@ i := [ps_na] -∗
    transaction_hpool_global_transferred trans -∗
    transaction_pagetable_entries_transferred i trans -∗
-   retrieval_entries i trans -∗
+   retrieval_entries_transferred i trans -∗
    R0 @@ V0 ->r encode_hvc_func Run -∗
    R1 @@ V0 ->r encode_vmid i -∗
    RX_state@i:= rx_state -∗
@@ -68,13 +69,14 @@ Lemma ftlr_nop {i trans' mem_acc_tx ai regs ps_acc p_tx p_rx ps_na instr} trans 
    VMProp i (vmprop_unknown i p_tx p_rx trans') 1 -∗
    transaction_pagetable_entries_owned i trans -∗
    pagetable_entries_excl_owned i (ps_acc ∖ {[p_rx; p_tx]} ∖ pages_in_trans trans) -∗
+   retrieval_entries_owned i trans -∗
    (∃ mem1 : mem, memory_pages ((ps_acc ∪ (pages_in_trans (trans_memory_in_trans i trans))) ∖ ps_acc) mem1) -∗
    ([∗ map] k↦v ∈ mem_acc_tx, k ->a v) -∗
    (∃ mem2 : mem, memory_page p_tx mem2) -∗
    SSWP ExecI @ i {{ bm, (if bm.1 then VMProp_holds i (1 / 2) else True) -∗ WP bm.2 @ i {{ _, True }} }}.
   Proof.
     iIntros (Htotal_regs Hsubset_mb Hdisj_na Hnin_rx Hnin_tx Hlookup_PC Hin_ps_acc Hneq_ptx Hdom_mem_acc_tx Hin_ps_acc_tx Hlookup_mem_ai Heqn).
-    iIntros "IH regs tx pgt_tx pgt_acc pgt_acc' LB trans_hpool_global tran_pgt_transferred retri R0z R1z rx_state rx prop0 propi tran_pgt_owned pgt_owned mem_rest mem_acc_tx mem_tx".
+    iIntros "IH regs tx pgt_tx pgt_acc pgt_acc' LB trans_hpool_global tran_pgt_transferred retri R0z R1z rx_state rx prop0 propi tran_pgt_owned pgt_owned retri_owned mem_rest mem_acc_tx mem_tx".
     (* getting the PC *)
     iDestruct (reg_big_sepM_split_upd i Hlookup_PC with "[$regs]")
       as "[PC Hacc_regs]";first done.
@@ -89,7 +91,7 @@ Lemma ftlr_nop {i trans' mem_acc_tx ai regs ps_acc p_tx p_rx ps_na instr} trans 
     iDestruct ("Hacc_mem_acc" with "[$mem_instr]") as "mem_acc_tx".
     iApply ("IH" $! _ ps_acc trans _ Htotal_regs' Hsubset_mb Hdisj_na Hnin_rx Hnin_tx with "regs tx pgt_tx pgt_acc pgt_acc'
                        LB trans_hpool_global tran_pgt_transferred retri R0z R1z rx_state rx prop0 propi
-                           tran_pgt_owned pgt_owned [mem_rest mem_acc_tx mem_tx]").
+                           tran_pgt_owned pgt_owned retri_owned [mem_rest mem_acc_tx mem_tx]").
     {
       iDestruct (memory_pages_split_singleton' p_tx ps_acc with "[mem_acc_tx $mem_tx]") as "mem_acc". set_solver + Hsubset_mb.
       iExists mem_acc_tx;by iFrame "mem_acc_tx".
