theories/logrel/ftlr_retrieve.v
@@ -44,7 +44,7 @@ Lemma ftlr_retrieve {i trans' mem_acc_tx ai regs ps_acc p_tx p_rx ps_na instr tr
                       LB@ i := [ps_na] -∗
                       transaction_hpool_global_transferred a1 -∗
                       transaction_pagetable_entries_transferred i a1 -∗
-                      retrieval_entries i a1 -∗
+                      retrieval_entries_transferred i a1 -∗
                       R0 @@ V0 ->r encode_hvc_func Run -∗
                       R1 @@ V0 ->r encode_vmid i -∗
                       RX_state@i:= a2 -∗
@@ -53,6 +53,7 @@ Lemma ftlr_retrieve {i trans' mem_acc_tx ai regs ps_acc p_tx p_rx ps_na instr tr
                       VMProp i (vmprop_unknown i p_tx p_rx trans') 1 -∗
                       transaction_pagetable_entries_owned i a1 -∗
                       pagetable_entries_excl_owned i (a0 ∖ {[p_rx; p_tx]} ∖ pages_in_trans a1) -∗
+                      retrieval_entries_owned i a1 -∗
                       (∃ mem : lang.mem, memory_pages (a0 ∪ pages_in_trans (trans_memory_in_trans i a1)) mem) -∗
                       WP ExecI @ i {{ _, True }}) -∗
    ([∗ map] r↦w ∈ regs, r @@ i ->r w) -∗
@@ -63,7 +64,7 @@ Lemma ftlr_retrieve {i trans' mem_acc_tx ai regs ps_acc p_tx p_rx ps_na instr tr
    LB@ i := [ps_na] -∗
    transaction_hpool_global_transferred trans -∗
    transaction_pagetable_entries_transferred i trans -∗
-   retrieval_entries i trans -∗
+   retrieval_entries_transferred i trans -∗
    R0 @@ V0 ->r encode_hvc_func Run -∗
    R1 @@ V0 ->r encode_vmid i -∗
    RX_state@i:= rx_state -∗
@@ -72,6 +73,7 @@ Lemma ftlr_retrieve {i trans' mem_acc_tx ai regs ps_acc p_tx p_rx ps_na instr tr
    VMProp i (vmprop_unknown i p_tx p_rx trans') 1 -∗
    transaction_pagetable_entries_owned i trans -∗
    pagetable_entries_excl_owned i (ps_acc ∖ {[p_rx; p_tx]} ∖ pages_in_trans trans) -∗
+   retrieval_entries_owned i trans -∗
    (∃ mem1 : mem, memory_pages ((ps_acc ∪ (pages_in_trans (trans_memory_in_trans i trans))) ∖ ps_acc) mem1) -∗
    ([∗ map] k↦v ∈ mem_acc_tx, k ->a v) -∗
    (∃ mem2 : mem, memory_page p_tx mem2) -∗
@@ -80,7 +82,7 @@ Lemma ftlr_retrieve {i trans' mem_acc_tx ai regs ps_acc p_tx p_rx ps_na instr tr
     iIntros (Htotal_regs Hsubset_mb Hneq_0 Hdisj_na Hnin_rx Hnin_tx Hlookup_PC Hin_ps_acc Hneq_ptx Hdom_mem_acc_tx Hin_ps_acc_tx
                          Hlookup_mem_ai Heqn  Hlookup_reg_R0 Hdecode_hvc).
     iIntros (Hneq_mb) "IH regs tx pgt_tx pgt_acc pgt_acc' LB trans_hpool_global tran_pgt_transferred retri R0z R1z rx_state rx prop0
-             propi tran_pgt_owned pgt_owned mem_rest mem_acc_tx mem_tx".
+             propi tran_pgt_owned pgt_owned retri_owned mem_rest mem_acc_tx mem_tx".
     set ps_mem_in_trans := (pages_in_trans (trans_memory_in_trans i trans)).
     pose proof (Htotal_regs R1) as[r1 Hlookup_reg_R1].
     pose proof (Htotal_regs R2) as[r2 Hlookup_reg_R2].
@@ -125,7 +127,7 @@ Lemma ftlr_retrieve {i trans' mem_acc_tx ai regs ps_acc p_tx p_rx ps_na instr tr
     }
 
     iDestruct (big_sepFM_lookup_Some Hlookup_tran with "retri'") as "[re' retri']".
-    simpl;left;split;done.
+    simpl. split;auto.
     rewrite Heq_retri.
     iDestruct (retri_split with "[$re $re']") as "re".
 
@@ -169,22 +171,37 @@ Lemma ftlr_retrieve {i trans' mem_acc_tx ai regs ps_acc p_tx p_rx ps_na instr tr
         set_solver +.
     }
 
+    assert(tran.1 = (tran.1.1.1.1.1, tran.1.1.1.1.2, i, tran.1.1.2, tran.1.2)) as Hrw_tran.
+    {
+      rewrite -Heq_tran.
+      repeat destruct tran as [tran ?]. simpl. done.
+    }
+    rewrite Hrw_tran.
+
     destruct (tran.1.2) eqn:Heq_tran_tt.
-    { (*apply [hvc_mem_retrieve_donate]*)
+    { (* retrieve donate*)
       iDestruct (big_sepFM_lookup_Some Hlookup_tran with "tran_pgt_transferred") as "[[tran' [own_tran excl_tran]] tran_pgt_transferred]".
       simpl. split;first done. left;done.
+      rewrite Hrw_tran; clear Hrw_tran.
       iDestruct (trans_split with "[$tran $tran']") as "tran".
 
-      destruct Hlookup_mem_ai as [Hlookup_mem_ai|Hlookup_mem_ai].
+      assert (pages_in_trans (trans_memory_in_trans i (delete r1 trans)) = ps_mem_in_trans ∖ tran.1.1.2) as Hrewrite.
       {
+        rewrite /trans_memory_in_trans.
+        rewrite map_filter_delete.
+        apply pages_in_trans_delete.
+        rewrite map_filter_lookup_Some.
+        split;first done.
+        simpl. right. done.
+        apply (trans_ps_disj_subseteq trans).
+        done.
+        apply map_filter_subseteq.
+      }
+
+
+      destruct Hlookup_mem_ai as [Hlookup_mem_ai|Hlookup_mem_ai].
+      { (* apply [hvc_mem_retrieve_donate]*)
         iDestruct (mem_big_sepM_split mem_acc_tx_rx Hlookup_mem_ai with "mem_acc_tx_rx") as "[mem_instr Hacc_mem_acc_tx_rx]".
-        assert(tran.1 = (tran.1.1.1.1.1, tran.1.1.1.1.2, i, tran.1.1.2, Donation)) as ?.
-        {
-          rewrite -Heq_tran_tt.
-          rewrite -Heq_tran.
-          repeat destruct tran as [tran ?]. simpl. done.
-        }
-        rewrite H; clear H.
 
         iApply (hvc_mem_retrieve_donate ai r1 with "[$PC $mem_instr $R0 $R1 $own_tran $pgt_acc $re $tran $rx $rx_state $mem_rx $fresh_handles]").
         set_solver + Hin_ps_acc_tx.
@@ -198,22 +215,9 @@ Lemma ftlr_retrieve {i trans' mem_acc_tx ai regs ps_acc p_tx p_rx ps_na instr tr
         iDestruct ("Hacc_mem_acc_tx_rx" with "[$mem_instr]") as "mem_acc_tx_rx".
         iDestruct (access_split with "pgt_acc") as "[pgt_acc pgt_acc']".
 
-        assert (pages_in_trans (trans_memory_in_trans i (delete r1 trans)) = ps_mem_in_trans ∖ tran.1.1.2) as Hrewrite.
-        {
-          rewrite /trans_memory_in_trans.
-          rewrite map_filter_delete.
-          apply pages_in_trans_delete.
-          rewrite map_filter_lookup_Some.
-          split;first done.
-          simpl. right. done.
-          apply (trans_ps_disj_subseteq trans).
-          done.
-          apply map_filter_subseteq.
-        }
-
         iApply ("IH" $! _ _ (delete r1 trans) _ Htotal_regs' _ _ _ _ with "regs tx pgt_tx pgt_acc pgt_acc' LB [fresh_handles trans]
                             [tran_pgt_transferred] [retri retri'] R0z R1z rx_state [$rx $pgt_rx] prop0 propi [tran_pgt_owned]
-                            [own_tran excl_tran pgt_owned] [mem_rest mem_acc_tx_rx mem_rx mem_tx]").
+                            [own_tran excl_tran pgt_owned] [retri_owned] [mem_rest mem_acc_tx_rx mem_rx mem_tx]").
         {
           iExists (hpool ∪ {[r1]}).
           iFrame "fresh_handles trans".
@@ -242,8 +246,282 @@ Lemma ftlr_retrieve {i trans' mem_acc_tx ai regs ps_acc p_tx p_rx ps_na instr tr
           done.
         }
         {
-          rewrite /retrieval_entries.
+          rewrite /retrieval_entries_transferred.
           iFrame "retri retri'".
+        }
+        {
+          rewrite /transaction_pagetable_entries_owned.
+          rewrite (big_sepFM_delete_False Hlookup_tran).
+          iFrame "tran_pgt_owned".
+          simpl.
+          intros [_ ?].
+          contradiction.
+        }
+        {
+          assert (pages_in_trans (delete r1 trans) = pages_in_trans trans ∖ tran.1.1.2) as ->.
+          {
+            apply pages_in_trans_delete;auto.
+          }
+          rewrite (difference_union_distr_l_L tran.1.1.2).
+          assert (tran.1.1.2 ∖ {[p_rx;p_tx]} = tran.1.1.2) as ->.
+          set_solver + Hnin_rx Hnin_tx Hsubseteq_tran.
+          rewrite (difference_union_distr_l_L tran.1.1.2).
+          assert (tran.1.1.2 ∖ (pages_in_trans trans ∖ tran.1.1.2) = tran.1.1.2) as ->.
+          set_solver + Hsubseteq_tran.
+          assert (ps_mem_in_trans ⊆ pages_in_trans trans) as Hsub.
+          apply pages_in_trans_subseteq.
+          apply map_filter_subseteq.
+          assert (tran.1.1.2 ∪ ps_acc ∖ {[p_rx; p_tx]} ∖ (pages_in_trans trans ∖ tran.1.1.2) = tran.1.1.2 ∪ ps_acc ∖ {[p_rx; p_tx]} ∖ pages_in_trans trans) as ->.
+          set A := (ps_acc ∖ {[p_rx; p_tx]}).
+          set G := (tran.1.1.2 ∪ A ∖ (pages_in_trans trans ∖ tran.1.1.2)).
+
+          rewrite (union_difference_L tran.1.1.2 (pages_in_trans trans) ).
+          2: {
+            set_solver + Hsub Hsubseteq_tran.
+          }
+          rewrite difference_union_distr_r_L.
+          rewrite union_intersection_l_L.
+          rewrite (union_comm_L tran.1.1.2).
+          rewrite difference_union_L.
+          rewrite intersection_comm_L.
+          symmetry.
+          rewrite /G.
+          rewrite subseteq_intersection_1_L. done.
+          set_solver +.
+          iDestruct "pgt_owned" as "[own_owned excl_owned]".
+          iSplitL "own_owned own_tran".
+          iApply (big_sepS_union with "[$own_tran $own_owned]").
+          set_solver + Hsubseteq_tran Hsub.
+          iApply (big_sepS_union with "[$excl_tran $excl_owned]").
+          set_solver + Hsubseteq_tran Hsub.
+        }
+        {
+          rewrite /retrieval_entries_owned.
+          rewrite -big_sepFM_delete_False;auto.
+          apply Hlookup_tran.
+          simpl.
+          intro; destruct H. rewrite Heq_retri // in H0.
+        }
+        {
+          rewrite Hrewrite.
+          rewrite (union_comm_L tran.1.1.2).
+          rewrite -(union_assoc_L ps_acc tran.1.1.2).
+          rewrite -(union_difference_L tran.1.1.2);last set_solver + Hsubseteq_tran.
+          iApply (memory_pages_split_diff' _ ps_acc).
+          set_solver +.
+          iSplitL "mem_rest"; first done.
+          iDestruct (memory_pages_split_singleton' p_rx with "[mem_acc_tx_rx mem_rx]") as "mem_acc_tx". set_solver + Hsubset_mb.
+          iSplitL "mem_acc_tx_rx".
+          iExists mem_acc_tx_rx; by iFrame "mem_acc_tx_rx".
+          iExists (list_to_map (zip (finz.seq p_rx (length des)) des) ∪ mem_rx); by iFrame "mem_rx".
+          iApply (memory_pages_split_singleton' p_tx with "[$mem_acc_tx $mem_tx]"). set_solver + Hsubset_mb.
+        }
+      }
+      { (* apply [hvc_mem_retrieve_donate_rx]*)
+        iDestruct (mem_big_sepM_split mem_rx Hlookup_mem_ai with "[mem_rx]") as "[mem_instr Hacc_mem_rx]".
+        iDestruct "mem_rx" as "[? $]".
+        rewrite set_of_addr_singleton in Hdom_mem_rx.
+
+        assert (p_rx = (tpa ai)) as ->.
+        {
+          apply elem_of_dom_2 in Hlookup_mem_ai.
+          rewrite Hdom_mem_rx in Hlookup_mem_ai.
+          rewrite elem_of_list_to_set in Hlookup_mem_ai.
+          apply elem_of_addr_of_page_iff in Hlookup_mem_ai.
+          done.
+        }
+
+        iApply (hvc_mem_retrieve_donate_rx ai r1 with "[$PC $mem_instr $R0 $R1 $own_tran $pgt_acc $re $tran $rx $rx_state Hacc_mem_rx $fresh_handles]").
+        done.
+        done.
+        iNext. iIntros "ai". iDestruct ("Hacc_mem_rx" with "ai") as "rx".
+        iSplitL "". 2: iExact "rx". done.
+        iNext.
+        simpl.
+        iIntros "(PC & R0 & R1 & own_tran & pgt_acc & rx & (%wl & %des & rx_state & _ & _ & mem_rx) & fresh_handles) _".
+
+        iDestruct ("Hacc_regs" $! (ai ^+ 1)%f with "[$ PC $ R0 $ R1 $ R2]") as (regs') "[%Htotal_regs' regs]".
+        iDestruct (access_split with "pgt_acc") as "[pgt_acc pgt_acc']".
+
+
+        iApply ("IH" $! _ _ (delete r1 trans) _ Htotal_regs' _ _ _ _ with "regs tx pgt_tx pgt_acc pgt_acc' LB [fresh_handles trans]
+                            [tran_pgt_transferred] [retri retri'] R0z R1z rx_state [$rx $pgt_rx] prop0 propi [tran_pgt_owned]
+                            [own_tran excl_tran pgt_owned] [retri_owned] [mem_rest mem_acc_tx_rx mem_rx mem_tx]").
+        {
+          iExists (hpool ∪ {[r1]}).
+          iFrame "fresh_handles trans".
+          iPureIntro.
+          assert (r1 ∈ dom (gset _) trans).
+          {
+            rewrite elem_of_dom.
+            exists tran;done.
+          }
+          rewrite union_comm_L in Heq_hsall.
+          rewrite -Heq_hsall.
+          rewrite union_comm_L.
+          rewrite (union_comm_L hpool).
+          rewrite union_assoc_L.
+          f_equal.
+          rewrite dom_delete_L.
+          rewrite difference_union_L.
+          split.
+          set_solver + H.
+          apply (trans_ps_disj_subseteq trans).
+          done.
+          apply map_subseteq_delete.
+        }
+        {
+          rewrite /transaction_pagetable_entries_transferred.
+          done.
+        }
+        {
+          rewrite /retrieval_entries_transferred.
+          iFrame "retri retri'".
+        }
+        {
+          rewrite /transaction_pagetable_entries_owned.
+          rewrite (big_sepFM_delete_False Hlookup_tran).
+          iFrame "tran_pgt_owned".
+          simpl.
+          intros [_ ?].
+          contradiction.
+        }
+        {
+          assert (pages_in_trans (delete r1 trans) = pages_in_trans trans ∖ tran.1.1.2) as ->.
+          {
+            apply pages_in_trans_delete;auto.
+          }
+          rewrite (difference_union_distr_l_L tran.1.1.2).
+          assert (tran.1.1.2 ∖ {[(tpa ai);p_tx]} = tran.1.1.2) as ->.
+          set_solver + Hnin_rx Hnin_tx Hsubseteq_tran.
+          rewrite (difference_union_distr_l_L tran.1.1.2).
+          assert (tran.1.1.2 ∖ (pages_in_trans trans ∖ tran.1.1.2) = tran.1.1.2) as ->.
+          set_solver + Hsubseteq_tran.
+          assert (ps_mem_in_trans ⊆ pages_in_trans trans) as Hsub.
+          apply pages_in_trans_subseteq.
+          apply map_filter_subseteq.
+          assert (tran.1.1.2 ∪ ps_acc ∖ {[(tpa ai); p_tx]} ∖ (pages_in_trans trans ∖ tran.1.1.2) = tran.1.1.2 ∪ ps_acc ∖ {[(tpa ai); p_tx]} ∖ pages_in_trans trans) as ->.
+          set A := (ps_acc ∖ {[(tpa ai); p_tx]}).
+          set G := (tran.1.1.2 ∪ A ∖ (pages_in_trans trans ∖ tran.1.1.2)).
+
+          rewrite (union_difference_L tran.1.1.2 (pages_in_trans trans) ).
+          2: {
+            set_solver + Hsub Hsubseteq_tran.
+          }
+          rewrite difference_union_distr_r_L.
+          rewrite union_intersection_l_L.
+          rewrite (union_comm_L tran.1.1.2).
+          rewrite difference_union_L.
+          rewrite intersection_comm_L.
+          symmetry.
+          rewrite /G.
+          rewrite subseteq_intersection_1_L. done.
+          set_solver +.
+          iDestruct "pgt_owned" as "[own_owned excl_owned]".
+          iSplitL "own_owned own_tran".
+          iApply (big_sepS_union with "[$own_tran $own_owned]").
+          set_solver + Hsubseteq_tran Hsub.
+          iApply (big_sepS_union with "[$excl_tran $excl_owned]").
+          set_solver + Hsubseteq_tran Hsub.
+        }
+        {
+          rewrite /retrieval_entries_owned.
+          rewrite -big_sepFM_delete_False;auto.
+          apply Hlookup_tran.
+          simpl.
+          intro; destruct H. rewrite Heq_retri // in H0. 
+        }
+        {
+          rewrite Hrewrite.
+          rewrite (union_comm_L tran.1.1.2).
+          rewrite -(union_assoc_L ps_acc tran.1.1.2).
+          rewrite -(union_difference_L tran.1.1.2);last set_solver + Hsubseteq_tran.
+          iApply (memory_pages_split_diff' _ ps_acc).
+          set_solver +.
+          iSplitL "mem_rest"; first done.
+          iDestruct (memory_pages_split_singleton' (tpa ai) with "[mem_acc_tx_rx mem_rx]") as "mem_acc_tx". set_solver + Hsubset_mb.
+          iSplitL "mem_acc_tx_rx".
+          iExists mem_acc_tx_rx; by iFrame "mem_acc_tx_rx".
+          iExists (list_to_map (zip (finz.seq (tpa ai) (length des)) des) ∪ mem_rx); by iFrame "mem_rx".
+          iApply (memory_pages_split_singleton' p_tx with "[$mem_acc_tx $mem_tx]"). set_solver + Hsubset_mb.
+        }
+      }
+    }
+    { (* retrieve share*)
+      clear Hrw_tran.
+      (* assert (pages_in_trans (trans_memory_in_trans i (delete r1 trans)) = ps_mem_in_trans ∖ tran.1.1.2) as Hrewrite. *)
+      (* { *)
+      (*   rewrite /trans_memory_in_trans. *)
+      (*   rewrite map_filter_delete. *)
+      (*   apply pages_in_trans_delete. *)
+      (*   rewrite map_filter_lookup_Some. *)
+      (*   split;first done. *)
+      (*   simpl. right. done. *)
+      (*   apply (trans_ps_disj_subseteq trans). *)
+      (*   done. *)
+      (*   apply map_filter_subseteq. *)
+      (* } *)
+
+      destruct Hlookup_mem_ai as [Hlookup_mem_ai|Hlookup_mem_ai].
+      { (* apply [hvc_mem_retrieve_share]*)
+        iDestruct (mem_big_sepM_split mem_acc_tx_rx Hlookup_mem_ai with "mem_acc_tx_rx") as "[mem_instr Hacc_mem_acc_tx_rx]".
+
+        iApply (hvc_mem_retrieve_share ai r1 with "[$PC $mem_instr $R0 $R1 $pgt_acc $re $tran $rx $rx_state $mem_rx]").
+        set_solver + Hin_ps_acc_tx.
+        done.
+        done.
+        iNext.
+        simpl.
+        iIntros "(PC & mem_instr & R0 & R1 & pgt_acc & re & tran & rx & (%wl & %des & rx_state & _ & _ & mem_rx)) _".
+
+        iDestruct ("Hacc_regs" $! (ai ^+ 1)%f with "[$ PC $ R0 $ R1 $ R2]") as (regs') "[%Htotal_regs' regs]".
+        iDestruct ("Hacc_mem_acc_tx_rx" with "[$mem_instr]") as "mem_acc_tx_rx".
+        iDestruct (access_split with "pgt_acc") as "[pgt_acc pgt_acc']".
+
+        iDestruct (retri_split with "re") as "[re re']".
+
+        iApply ("IH" $! _ _ (<[r1 := (tran.1, true)]> trans) _ Htotal_regs' _ _ _ _ with "regs tx pgt_tx pgt_acc pgt_acc' LB
+                            [fresh_handles trans tran]
+                            [tran_pgt_transferred] [retri retri' re] R0z R1z rx_state [$rx $pgt_rx] prop0 propi [tran_pgt_owned]
+                            [pgt_owned] [retri_owned re'] [mem_rest mem_acc_tx_rx mem_rx mem_tx]").
+        (* TODO *)
+        {
+          iExists (hpool ∪ {[r1]}).
+          iFrame "fresh_handles trans".
+          iPureIntro.
+          assert (r1 ∈ dom (gset _) trans).
+          {
+            rewrite elem_of_dom.
+            exists tran;done.
+          }
+          rewrite union_comm_L in Heq_hsall.
+          rewrite -Heq_hsall.
+          rewrite union_comm_L.
+          rewrite (union_comm_L hpool).
+          rewrite union_assoc_L.
+          f_equal.
+          rewrite dom_delete_L.
+          rewrite difference_union_L.
+          split.
+          set_solver + H.
+          apply (trans_ps_disj_subseteq trans).
+          done.
+          apply map_subseteq_delete.
+        }
+        {
+          rewrite /transaction_pagetable_entries_transferred.
+          done.
+        }
+        {
+          rewrite /retrieval_entries_transferred.
+
+        (* iDestruct (big_sepFM_delete_acc_True (tran.1, true) with "retri") as "retri". *)
+        (* simpl. left;done. *)
+        (* iDestruct (big_sepFM_delete_acc_False (tran.1, true) with "retri'") as "retri'". *)
+        (* simpl. admit. *)
+        (*TODO: tran.1.1.1.1.1 ≠ tran.1.1.1.2? *)
+          iFrame "retri retri'".
+
         }
         {
           rewrite /transaction_pagetable_entries_owned.
@@ -307,11 +585,127 @@ Lemma ftlr_retrieve {i trans' mem_acc_tx ai regs ps_acc p_tx p_rx ps_na instr tr
         }
       }
       { (* apply [hvc_mem_retrieve_donate_rx]*)
-        admit.
+        iDestruct (mem_big_sepM_split mem_rx Hlookup_mem_ai with "[mem_rx]") as "[mem_instr Hacc_mem_rx]".
+        iDestruct "mem_rx" as "[? $]".
+        rewrite set_of_addr_singleton in Hdom_mem_rx.
+
+        assert (p_rx = (tpa ai)) as ->.
+        {
+          apply elem_of_dom_2 in Hlookup_mem_ai.
+          rewrite Hdom_mem_rx in Hlookup_mem_ai.
+          rewrite elem_of_list_to_set in Hlookup_mem_ai.
+          apply elem_of_addr_of_page_iff in Hlookup_mem_ai.
+          done.
+        }
+
+        iApply (hvc_mem_retrieve_donate_rx ai r1 with "[$PC $mem_instr $R0 $R1 $own_tran $pgt_acc $re $tran $rx $rx_state Hacc_mem_rx $fresh_handles]").
+        done.
+        done.
+        iNext. iIntros "ai". iDestruct ("Hacc_mem_rx" with "ai") as "rx".
+        iSplitL "". 2: iExact "rx". done.
+        iNext.
+        simpl.
+        iIntros "(PC & R0 & R1 & own_tran & pgt_acc & rx & (%wl & %des & rx_state & _ & _ & mem_rx) & fresh_handles) _".
+
+        iDestruct ("Hacc_regs" $! (ai ^+ 1)%f with "[$ PC $ R0 $ R1 $ R2]") as (regs') "[%Htotal_regs' regs]".
+        iDestruct (access_split with "pgt_acc") as "[pgt_acc pgt_acc']".
+
+
+        iApply ("IH" $! _ _ (delete r1 trans) _ Htotal_regs' _ _ _ _ with "regs tx pgt_tx pgt_acc pgt_acc' LB [fresh_handles trans]
+                            [tran_pgt_transferred] [retri retri'] R0z R1z rx_state [$rx $pgt_rx] prop0 propi [tran_pgt_owned]
+                            [own_tran excl_tran pgt_owned] [mem_rest mem_acc_tx_rx mem_rx mem_tx]").
+        {
+          iExists (hpool ∪ {[r1]}).
+          iFrame "fresh_handles trans".
+          iPureIntro.
+          assert (r1 ∈ dom (gset _) trans).
+          {
+            rewrite elem_of_dom.
+            exists tran;done.
+          }
+          rewrite union_comm_L in Heq_hsall.
+          rewrite -Heq_hsall.
+          rewrite union_comm_L.
+          rewrite (union_comm_L hpool).
+          rewrite union_assoc_L.
+          f_equal.
+          rewrite dom_delete_L.
+          rewrite difference_union_L.
+          split.
+          set_solver + H.
+          apply (trans_ps_disj_subseteq trans).
+          done.
+          apply map_subseteq_delete.
+        }
+        {
+          rewrite /transaction_pagetable_entries_transferred.
+          done.
+        }
+        {
+          rewrite /retrieval_entries_transferred.
+          iFrame "retri retri'".
+        }
+        {
+          rewrite /transaction_pagetable_entries_owned.
+          rewrite (big_sepFM_delete_False Hlookup_tran).
+          iFrame "tran_pgt_owned".
+          simpl.
+          intros [_ ?].
+          contradiction.
+        }
+        {
+          assert (pages_in_trans (delete r1 trans) = pages_in_trans trans ∖ tran.1.1.2) as ->.
+          {
+            apply pages_in_trans_delete;auto.
+          }
+          rewrite (difference_union_distr_l_L tran.1.1.2).
+          assert (tran.1.1.2 ∖ {[(tpa ai);p_tx]} = tran.1.1.2) as ->.
+          set_solver + Hnin_rx Hnin_tx Hsubseteq_tran.
+          rewrite (difference_union_distr_l_L tran.1.1.2).
+          assert (tran.1.1.2 ∖ (pages_in_trans trans ∖ tran.1.1.2) = tran.1.1.2) as ->.
+          set_solver + Hsubseteq_tran.
+          assert (ps_mem_in_trans ⊆ pages_in_trans trans) as Hsub.
+          apply pages_in_trans_subseteq.
+          apply map_filter_subseteq.
+          assert (tran.1.1.2 ∪ ps_acc ∖ {[(tpa ai); p_tx]} ∖ (pages_in_trans trans ∖ tran.1.1.2) = tran.1.1.2 ∪ ps_acc ∖ {[(tpa ai); p_tx]} ∖ pages_in_trans trans) as ->.
+          set A := (ps_acc ∖ {[(tpa ai); p_tx]}).
+          set G := (tran.1.1.2 ∪ A ∖ (pages_in_trans trans ∖ tran.1.1.2)).
+
+          rewrite (union_difference_L tran.1.1.2 (pages_in_trans trans) ).
+          2: {
+            set_solver + Hsub Hsubseteq_tran.
+          }
+          rewrite difference_union_distr_r_L.
+          rewrite union_intersection_l_L.
+          rewrite (union_comm_L tran.1.1.2).
+          rewrite difference_union_L.
+          rewrite intersection_comm_L.
+          symmetry.
+          rewrite /G.
+          rewrite subseteq_intersection_1_L. done.
+          set_solver +.
+          iDestruct "pgt_owned" as "[own_owned excl_owned]".
+          iSplitL "own_owned own_tran".
+          iApply (big_sepS_union with "[$own_tran $own_owned]").
+          set_solver + Hsubseteq_tran Hsub.
+          iApply (big_sepS_union with "[$excl_tran $excl_owned]").
+          set_solver + Hsubseteq_tran Hsub.
+        }
+        {
+          rewrite Hrewrite.
+          rewrite (union_comm_L tran.1.1.2).
+          rewrite -(union_assoc_L ps_acc tran.1.1.2).
+          rewrite -(union_difference_L tran.1.1.2);last set_solver + Hsubseteq_tran.
+          iApply (memory_pages_split_diff' _ ps_acc).
+          set_solver +.
+          iSplitL "mem_rest"; first done.
+          iDestruct (memory_pages_split_singleton' (tpa ai) with "[mem_acc_tx_rx mem_rx]") as "mem_acc_tx". set_solver + Hsubset_mb.
+          iSplitL "mem_acc_tx_rx".
+          iExists mem_acc_tx_rx; by iFrame "mem_acc_tx_rx".
+          iExists (list_to_map (zip (finz.seq (tpa ai) (length des)) des) ∪ mem_rx); by iFrame "mem_rx".
+          iApply (memory_pages_split_singleton' p_tx with "[$mem_acc_tx $mem_tx]"). set_solver + Hsubset_mb.
+        }
       }
-    }
-    { (* apply [hvc_mem_retrieve_share]*)
-      admit.
     }
     { (*apply [hvc_mem_retrieve_lend]*)
       admit.
